sampling p-f

proofs/fstar/extraction-edited/Libcrux.Kem.Kyber.Sampling.fst
@@ -4,17 +4,18 @@ open Core
 open FStar.Mul
 
 let rejection_sampling_panic_with_diagnostic () : Prims.unit =
-  admit(); // This should never happen
+  admit(); // This should never be reachable
   Rust_primitives.Hax.never_to_any (Core.Panicking.panic "explicit panic"
       <:
       Rust_primitives.Hax.t_Never)
 
+#push-options "--ifuel 0 --z3rlimit 100"
 let sample_from_binomial_distribution_2_ (randomness: t_Slice u8) =
-  let sampled = 
-    Libcrux.Kem.Kyber.Arithmetic.impl__PolynomialRingElement__ZERO
+  let sampled: t_PolynomialRingElement_b 3 = 
+    cast_poly_b Libcrux.Kem.Kyber.Arithmetic.impl__PolynomialRingElement__ZERO
   in
 
-  let acc_t = Libcrux.Kem.Kyber.Arithmetic.wfPolynomialRingElement in
+  let acc_t = Libcrux.Kem.Kyber.Arithmetic.t_PolynomialRingElement_b 3 in
   [@ inline_let]
   let inv = fun (acc:acc_t) (i:usize) -> True in
   let sl : t_Slice u8 = randomness in
@@ -22,14 +23,12 @@ let sample_from_binomial_distribution_2_ (randomness: t_Slice u8) =
   assert (v (length sl) == 128);
   assert (Seq.length sl == 128);
   assert_norm (128 % 4 == 0);
-  admit();
-  let sampled:Libcrux.Kem.Kyber.Arithmetic.wfPolynomialRingElement =
+  let sampled =
    Rust_primitives.Iterators.foldi_chunks_exact #u8 #acc_t #inv
       sl
       chunk_len
       sampled
       (fun sampled temp_1_ ->
-          let sampled:Libcrux.Kem.Kyber.Arithmetic.wfPolynomialRingElement = sampled in
           let chunk_number, byte_chunk:(usize & t_Array u8 chunk_len) = temp_1_ in
           assert(chunk_number <. sz 32);
           let (random_bits_as_u32: u32):u32 =
@@ -43,11 +42,13 @@ let sample_from_binomial_distribution_2_ (randomness: t_Slice u8) =
             ((cast (byte_chunk.[ sz 3 ] <: u8) <: u32) <<! 24l <: u32)
           in
           let even_bits:u32 = random_bits_as_u32 &. 1431655765ul in
-          assume(even_bits <=. 1431655765ul);
+          logand_lemma random_bits_as_u32 1431655765ul;
+          assert(even_bits <=. 1431655765ul);
           let odd_bits:u32 = (random_bits_as_u32 >>! 1l <: u32) &. 1431655765ul in
-          assume(odd_bits <=. 1431655765ul);
+          logand_lemma (random_bits_as_u32 >>! 1l <: u32) 1431655765ul;
+          assert(odd_bits <=. 1431655765ul);
           let coin_toss_outcomes:u32 = even_bits +! odd_bits in
-          let acc_t = Libcrux.Kem.Kyber.Arithmetic.wfPolynomialRingElement in
+          let acc_t = Libcrux.Kem.Kyber.Arithmetic.t_PolynomialRingElement_b 3 in
           [@ inline_let]
           let inv : acc_t -> u32 -> Type = fun acc i -> True in
             Rust_primitives.Iterators.foldi_range_step_by #u32_inttype #(acc_t) #inv ({
@@ -59,24 +60,40 @@ let sample_from_binomial_distribution_2_ (randomness: t_Slice u8) =
             (sz 4)
             sampled
             (fun sampled outcome_set ->
-                let sampled:Libcrux.Kem.Kyber.Arithmetic.wfPolynomialRingElement = sampled in
                 let outcome_set:u32 = outcome_set in
+                assert (v outcome_set + 4 <= 32);
+                let out_1 = ((coin_toss_outcomes >>! outcome_set <: u32) &. 3ul <: u32) in
                 let outcome_1_:i32 =
-                  cast ((coin_toss_outcomes >>! outcome_set <: u32) &. 3ul <: u32) <: i32
+                  cast out_1  <: i32
                 in
+                let out_2 = ((coin_toss_outcomes >>! (outcome_set +! 2ul <: u32) <: u32) &. 3ul <: u32) in
                 let outcome_2_:i32 =
-                  cast ((coin_toss_outcomes >>! (outcome_set +! 2ul <: u32) <: u32) &. 3ul <: u32)
-                  <:
-                  i32
+                  cast out_2  <: i32
                 in
-                assume (outcome_1_ >=. 0l /\ outcome_1_ <. 3l);
-                assume (outcome_2_ >=. 0l /\ outcome_2_ <. 3l);
+                logand_lemma (coin_toss_outcomes >>! outcome_set <: u32) 3ul;
+                assert (v out_1 >= 0);
+                assert (v out_1 <= 3);
+                assert (v outcome_1_ == v out_1 @% pow2 32);
+                Math.Lemmas.small_modulo_lemma_1 (v out_1) (pow2 32);
+                assert (v outcome_1_ == v out_1);
+                assert (v outcome_1_ >= 0 /\ v outcome_1_ <= 3);
+                logand_lemma (coin_toss_outcomes >>! (outcome_set +! 2ul <: u32) <: u32) 3ul;
+                assert (v out_2 >= 0);
+                assert (v out_2 <= 3);
+                assert (v outcome_2_ == v out_2 @% pow2 32);
+                Math.Lemmas.small_modulo_lemma_1 (v out_2) (pow2 32);
+                assert (v outcome_2_ == v out_2);
+                assert (v outcome_2_ >= 0 /\ v outcome_2_ <= 3);
                 let offset:usize = cast (outcome_set >>! 2l <: u32) <: usize in
                 assert (outcome_set <. 32ul);
-                assume (offset <. sz 8);
+                assert (v (outcome_set >>! 2l <: u32) = v outcome_set / 4);
+                assert (v (outcome_set >>! 2l <: u32) < 8);
+                Math.Lemmas.small_modulo_lemma_1 (v (outcome_set >>! 2l <: u32)) (pow2 32);
+                Math.Lemmas.small_modulo_lemma_1 (v (outcome_set >>! 2l <: u32)) (pow2 64);
+                assert (v offset < 8);
                 assert (8 * v chunk_number + 8 <= 256);
                 assert (8 * v chunk_number + v offset < 256);
-                let sampled:Libcrux.Kem.Kyber.Arithmetic.wfPolynomialRingElement =
+                let sampled:Libcrux.Kem.Kyber.Arithmetic.t_PolynomialRingElement_b 3 =
                   {
                     sampled with
                     Libcrux.Kem.Kyber.Arithmetic.f_coefficients
@@ -87,20 +104,21 @@ let sample_from_binomial_distribution_2_ (randomness: t_Slice u8) =
                       (outcome_1_ -! outcome_2_ <: i32)
                   }
                   <:
-                  Libcrux.Kem.Kyber.Arithmetic.wfPolynomialRingElement
+                  Libcrux.Kem.Kyber.Arithmetic.t_PolynomialRingElement_b 3
                 in
                 sampled))
-  in
-  let _:Prims.unit = () <: Prims.unit in
+  in 
+  let _:Prims.unit = () <: Prims.unit in 
   admit(); // P-F
   sampled 
+#pop-options
 
+#push-options "--ifuel 0 --z3rlimit 200"
 let sample_from_binomial_distribution_3_ (randomness: t_Slice u8) =
-  let (sampled: Libcrux.Kem.Kyber.Arithmetic.wfPolynomialRingElement):Libcrux.Kem.Kyber.Arithmetic.wfPolynomialRingElement
-  =
+  let sampled:t_PolynomialRingElement_b 7 =
     (Libcrux.Kem.Kyber.Arithmetic.cast_poly_b Libcrux.Kem.Kyber.Arithmetic.impl__PolynomialRingElement__ZERO)
   in
-  let acc_t = Libcrux.Kem.Kyber.Arithmetic.wfPolynomialRingElement in
+  let acc_t = Libcrux.Kem.Kyber.Arithmetic.t_PolynomialRingElement_b 7 in
   [@ inline_let]
   let inv = fun (acc:acc_t) (i:usize) -> True in
   let sl : t_Slice u8 = randomness in
@@ -108,13 +126,13 @@ let sample_from_binomial_distribution_3_ (randomness: t_Slice u8) =
   assert (v (length sl) == 192);
   assert (Seq.length sl == 192);
   assert_norm (192 % 3 == 0);
-  let sampled:Libcrux.Kem.Kyber.Arithmetic.wfPolynomialRingElement =
+  let sampled:Libcrux.Kem.Kyber.Arithmetic.t_PolynomialRingElement_b 7 =
    Rust_primitives.Iterators.foldi_chunks_exact #u8 #acc_t #inv
       sl
       chunk_len
       sampled
       (fun sampled temp_1_ ->
-          let sampled:Libcrux.Kem.Kyber.Arithmetic.wfPolynomialRingElement = sampled in
+          let sampled:Libcrux.Kem.Kyber.Arithmetic.t_PolynomialRingElement_b 7 = sampled in
           let chunk_number, byte_chunk:(usize & t_Array u8 chunk_len) = temp_1_ in
           let (random_bits_as_u24: u32):u32 =
             ((cast (byte_chunk.[ sz 0 ] <: u8) <: u32) |.
@@ -124,13 +142,16 @@ let sample_from_binomial_distribution_3_ (randomness: t_Slice u8) =
             ((cast (byte_chunk.[ sz 2 ] <: u8) <: u32) <<! 16l <: u32)
           in
           let first_bits:u32 = random_bits_as_u24 &. 2396745ul in
-          assume (first_bits <=. 2396745ul);
+          logand_lemma random_bits_as_u24 2396745ul;
+          assert (first_bits <=. 2396745ul);
           let second_bits:u32 = (random_bits_as_u24 >>! 1l <: u32) &. 2396745ul in
-          assume (second_bits <=. 2396745ul);
+          logand_lemma (random_bits_as_u24 >>! 1l <: u32) 2396745ul;
+          assert (second_bits <=. 2396745ul);
           let third_bits:u32 = (random_bits_as_u24 >>! 2l <: u32) &. 2396745ul in
-          assume (third_bits <=. 2396745ul);
+          logand_lemma (random_bits_as_u24 >>! 2l <: u32) 2396745ul;
+          assert (third_bits <=. 2396745ul);
           let coin_toss_outcomes:u32 = (first_bits +! second_bits <: u32) +! third_bits in
-          let acc_t = Libcrux.Kem.Kyber.Arithmetic.wfPolynomialRingElement in
+          let acc_t = Libcrux.Kem.Kyber.Arithmetic.t_PolynomialRingElement_b 7 in
           [@ inline_let]
           let inv : acc_t -> i32 -> Type = fun acc i -> True in
             Rust_primitives.Iterators.foldi_range_step_by #i32_inttype #(acc_t) #inv ({
@@ -142,7 +163,7 @@ let sample_from_binomial_distribution_3_ (randomness: t_Slice u8) =
             (sz 6)
             sampled
             (fun sampled outcome_set ->
-                let sampled:Libcrux.Kem.Kyber.Arithmetic.wfPolynomialRingElement = sampled in
+                let sampled:Libcrux.Kem.Kyber.Arithmetic.t_PolynomialRingElement_b 7 = sampled in
                 let outcome_set:i32 = outcome_set in
                 let outcome_1_:i32 =
                   cast ((coin_toss_outcomes >>! outcome_set <: u32) &. 7ul <: u32) <: i32
@@ -152,13 +173,22 @@ let sample_from_binomial_distribution_3_ (randomness: t_Slice u8) =
                   <:
                   i32
                 in
-                assume (outcome_1_ >=. 0l /\ outcome_1_ <. 7l);
-                assume (outcome_2_ >=. 0l /\ outcome_2_ <. 7l);
+                logand_lemma (coin_toss_outcomes >>! outcome_set <: u32) 7ul;
+                Math.Lemmas.small_modulo_lemma_1 (v ((coin_toss_outcomes >>! outcome_set <: u32) &. 7ul <: u32)) (pow2 32);
+                assert (v outcome_1_ >= 0 /\ v outcome_1_ <= 7);
+                logand_lemma (coin_toss_outcomes >>! (outcome_set +! 3l <: i32) <: u32) 7ul;
+                Math.Lemmas.small_modulo_lemma_1 (v ((coin_toss_outcomes >>! (outcome_set +! 3l <: i32) <: u32) &. 7ul <: u32)) (pow2 32);
+                assert (v outcome_2_ >= 0 /\ v outcome_2_ <= 7);
                 let offset:usize = cast (outcome_set /! 6l <: i32) <: usize in
-                assume(offset <. sz 4);
-                admit();
-                assert(4 * v chunk_number + v offset < 256);
-                let sampled:Libcrux.Kem.Kyber.Arithmetic.wfPolynomialRingElement =
+                assert (outcome_set <. 24l);
+                assert (v (outcome_set /! 6l <: i32) = v outcome_set / 6);
+                assert (v (outcome_set /! 6l <: i32) < 4);
+                Math.Lemmas.small_modulo_lemma_1 (v (outcome_set /! 6l <: i32)) (pow2 32);
+                Math.Lemmas.small_modulo_lemma_1 (v (outcome_set /! 6l <: i32)) (pow2 64);
+                assert (v offset < 4);
+                assert (4 * v chunk_number + 4 <= 256);
+                assert (4 * v chunk_number + v offset < 256);
+                let sampled:Libcrux.Kem.Kyber.Arithmetic.t_PolynomialRingElement_b 7 =
                   {
                     sampled with
                     Libcrux.Kem.Kyber.Arithmetic.f_coefficients
@@ -169,18 +199,18 @@ let sample_from_binomial_distribution_3_ (randomness: t_Slice u8) =
                       (outcome_1_ -! outcome_2_ <: i32)
                   }
                   <:
-                  Libcrux.Kem.Kyber.Arithmetic.wfPolynomialRingElement
+                  Libcrux.Kem.Kyber.Arithmetic.t_PolynomialRingElement_b 7
                 in
                 sampled))
   in
   let _:Prims.unit = () <: Prims.unit in
   admit();
   sampled
+#pop-options
 
 let sample_from_binomial_distribution (v_ETA: usize) (randomness: t_Slice u8) =
   let _:Prims.unit = () <: Prims.unit in
   Rust_primitives.Integers.mk_int_equiv_lemma #u32_inttype (v v_ETA);
-  admit();
   match cast (v_ETA <: usize) <: u32 with
   | 2ul -> sample_from_binomial_distribution_2_ randomness
   | 3ul -> sample_from_binomial_distribution_3_ randomness
@@ -223,9 +253,22 @@ let sample_from_uniform_distribution (randomness: t_Array u8 (sz 840)) =
             let b1:i32 = cast (bytes.[ sz 0 ] <: u8) <: i32 in
             let b2:i32 = cast (bytes.[ sz 1 ] <: u8) <: i32 in
             let b3:i32 = cast (bytes.[ sz 2 ] <: u8) <: i32 in
+            assert(v b1 >= 0 /\ v b1 < pow2 8);
+            assert(v b2 >= 0 /\ v b2 < pow2 8);
+            assert(v b3 >= 0 /\ v b3 < pow2 8);
             let d1:i32 = ((b2 &. 15l <: i32) <<! 8l <: i32) |. b1 in
+            assert (15 = pow2 4 - 1);
+            mk_int_equiv_lemma #i32_inttype 15;
+            assert (15l = mk_int (pow2 4) -! mk_int 1);
+            logand_mask_lemma b2 4;
+            assert (v ((b2 &. 15l <: i32) <<! 8l <: i32) == (v b2 % 16) * pow2 8);
+            logor_lemma ((b2 &. 15l <: i32) <<! 8l <: i32) b1;
+            assert (v d1 >= v b1);
+            assert (v d1 >= 0);
             let d2:i32 = (b3 <<! 4l <: i32) |. (b2 >>! 4l <: i32) in
-            admit();
+            logor_lemma (b3 <<! 4l <: i32) (b2 >>! 4l <: i32);
+            assert (v d2 >= v b3 * pow2 4);
+            assert (v d2 >= 0);
             let out, sampled_coefficients:(Libcrux.Kem.Kyber.Arithmetic.wfPolynomialRingElement &
               usize) =
               if
